Squash.
Start adding compartments to the recorded external calls

Correct last week's work following last week's discussion with Arthur

Add compartment in events for Cminor's small step semantics

Add calling compartment to call state.

Add compartments to the external call trace events for CminorSel

Add compartments to the external call trace events for RTL

Add compartments to the external call trace events for Csharpminor

Add compartments to the external call trace events for the semantics of CompCert C

Add compartments to the external call trace events for the semantics of Clight

some propagation for callstates

Port big-step semantics.

Couple of fixes.

Fix RTLGenproof.

Splitlongproof.

RTLtyping.

backend/Cminor.v
@@ -391,7 +391,7 @@ Inductive eval_exprlist: list expr -> list val -> Prop :=
 
 End EVAL_EXPR.
 
-(** Pop continuation until a call or stop *)
+(** Pop continuation until a call or stop while skipping tail frames *)
 
 Fixpoint call_cont (k: cont) : cont :=
   match k with
@@ -478,9 +478,10 @@ Inductive step: state -> trace -> state -> Prop :=
       step (State f (Stailcall sig a bl) k (Vptr sp Ptrofs.zero) e m)
         E0 (Callstate fd vargs f.(fn_comp) (call_cont k) m')
 
-  | step_builtin: forall f optid ef bl k sp e m vargs t vres m',
+  | step_builtin: forall f optid ef bl k sp e m c vargs t vres m',
       eval_exprlist sp e m bl vargs ->
-      external_call ef ge vargs m t vres m' ->
+      c = f.(fn_comp) ->
+      external_call ef ge c vargs m t vres m' ->
       step (State f (Sbuiltin optid ef bl) k sp e m)
          t (State f Sskip k sp (set_optvar optid vres e) m')
 
@@ -543,7 +544,7 @@ Inductive step: state -> trace -> state -> Prop :=
       step (Callstate (Internal f) vargs cp k m)
         E0 (State f f.(fn_body) k (Vptr sp Ptrofs.zero) e m')
   | step_external_function: forall ef cp vargs k m t vres m',
-      external_call ef ge vargs m t vres m' ->
+      external_call ef ge cp vargs m t vres m' ->
       step (Callstate (External ef) vargs cp k m)
          t (Returnstate vres k m')
 
@@ -641,7 +642,7 @@ Proof.
   intros. constructor; set (ge := Genv.globalenv p); simpl; intros.
 - (* determ *)
   inv H; inv H0; Determ.
-  + subst vargs0. exploit external_call_determ. eexact H2. eexact H13.
+  + subst vargs0. exploit external_call_determ. eexact H3.  eexact H14.
     intros (A & B). split; intros; auto.
     apply B in H; destruct H; congruence.
   + subst v0. assert (b0 = b) by (inv H2; inv H13; auto). subst b0; auto.
@@ -714,27 +715,28 @@ Section NATURALSEM.
 
 Variable ge: genv.
 
-(** Evaluation of a function invocation: [eval_funcall ge m f args t m' res]
+(** Evaluation of a function invocation: [eval_funcall ge cp m f args t m' res]
   means that the function [f], applied to the arguments [args] in
   memory state [m], returns the value [res] in modified memory state [m'].
   [t] is the trace of observable events generated during the invocation.
 *)
 
 Inductive eval_funcall:
+        compartment ->
         mem -> fundef -> list val -> trace ->
         mem -> val -> Prop :=
   | eval_funcall_internal:
-      forall m f vargs m1 sp e t e2 m2 out vres m3,
+      forall cp m f vargs m1 sp e t e2 m2 out vres m3,
       Mem.alloc m f.(fn_comp) 0 f.(fn_stackspace) = (m1, sp) ->
       set_locals f.(fn_vars) (set_params vargs f.(fn_params)) = e ->
       exec_stmt f (Vptr sp Ptrofs.zero) e m1 f.(fn_body) t e2 m2 out ->
       outcome_result_value out vres ->
       outcome_free_mem out m2 sp f.(fn_stackspace) m3 ->
-      eval_funcall m (Internal f) vargs t m3 vres
+      eval_funcall cp m (Internal f) vargs t m3 vres
   | eval_funcall_external:
-      forall ef m args t res m',
-      external_call ef ge args m t res m' ->
-      eval_funcall m (External ef) args t m' res
+      forall ef cp m args t res m',
+      external_call ef ge cp args m t res m' ->
+      eval_funcall cp m (External ef) args t m' res
 
 (** Execution of a statement: [exec_stmt ge f sp e m s t e' m' out]
   means that statement [s] executes with outcome [out].
@@ -767,13 +769,13 @@ with exec_stmt:
       eval_exprlist ge sp e m bl vargs ->
       Genv.find_funct ge vf = Some fd ->
       funsig fd = sig ->
-      eval_funcall m fd vargs t m' vres ->
+      eval_funcall f.(fn_comp) m fd vargs t m' vres ->
       e' = set_optvar optid vres e ->
       exec_stmt f sp e m (Scall optid sig a bl) t e' m' Out_normal
   | exec_Sbuiltin:
       forall f sp e m optid ef bl t m' vargs vres e',
       eval_exprlist ge sp e m bl vargs ->
-      external_call ef ge vargs m t vres m' ->
+      external_call ef ge f.(fn_comp) vargs m t vres m' ->
       e' = set_optvar optid vres e ->
       exec_stmt f sp e m (Sbuiltin optid ef bl) t e' m' Out_normal
   | exec_Sifthenelse:
@@ -832,7 +834,7 @@ with exec_stmt:
       funsig fd = sig ->
       forall (COMP: comp_of fd = f.(fn_comp)),
       Mem.free m sp 0 f.(fn_stackspace) = Some m' ->
-      eval_funcall m' fd vargs t m'' vres ->
+      eval_funcall f.(fn_comp) m' fd vargs t m'' vres ->
       exec_stmt f (Vptr sp Ptrofs.zero) e m (Stailcall sig a bl) t e m'' (Out_tailcall_return vres).
 
 Scheme eval_funcall_ind2 := Minimality for eval_funcall Sort Prop
@@ -923,7 +925,7 @@ Inductive bigstep_program_terminates (p: program): trace -> int -> Prop :=
       Genv.find_symbol ge p.(prog_main) = Some b ->
       Genv.find_funct_ptr ge b = Some f ->
       funsig f = signature_main ->
-      eval_funcall ge m0 f nil t m (Vint r) ->
+      eval_funcall ge default_compartment m0 f nil t m (Vint r) ->
       bigstep_program_terminates p t r.
 
 Inductive bigstep_program_diverges (p: program): traceinf -> Prop :=
@@ -987,9 +989,9 @@ Proof.
 Qed.
 
 Lemma eval_funcall_exec_stmt_steps:
-  (forall m fd args t m' res,
-   eval_funcall ge m fd args t m' res ->
-   forall cp k,
+  (forall cp m fd args t m' res,
+   eval_funcall ge cp m fd args t m' res ->
+   forall k,
    is_call_cont k ->
    star step ge (Callstate fd args cp k m)
               t (Returnstate res k m'))
@@ -1023,7 +1025,7 @@ Proof.
   reflexivity. traceEq.
 
 (* funcall external *)
-  apply star_one. constructor; auto.
+  apply star_one. econstructor; eauto.
 
 (* skip *)
   econstructor; split.
@@ -1149,9 +1151,9 @@ Proof.
 Qed.
 
 Lemma eval_funcall_steps:
-   forall m fd args t m' res,
-   eval_funcall ge m fd args t m' res ->
-   forall cp k,
+   forall cp m fd args t m' res,
+   eval_funcall ge cp m fd args t m' res ->
+   forall k,
    is_call_cont k ->
    star step ge (Callstate fd args cp k m)
               t (Returnstate res k m').
