backend/RTLtyping.v
@@ -855,9 +855,9 @@ Proof.
 Qed.
 
 Lemma wt_exec_Ibuiltin:
-  forall env f ef (ge: genv) args res s vargs m t vres m' rs,
+  forall env f ef (ge: genv) cp args res s vargs m t vres m' rs,
   wt_instr f env (Ibuiltin ef args res s) ->
-  external_call ef ge vargs m t vres m' ->
+  external_call ef ge cp vargs m t vres m' ->
   wt_regset env rs ->
   wt_regset env (regmap_setres res vres rs).
 Proof.
@@ -926,7 +926,7 @@ Lemma subject_reduction:
   forall (WT: wt_state st1), wt_state st2.
 Proof.
   induction 1; intros; inv WT;
-  try (generalize (wt_instrs _ _ WT_FN pc _ H); intros WTI).
+  try (exploit (wt_instrs _ _ WT_FN pc); eauto; intros WTI).
   (* Inop *)
   econstructor; eauto.
   (* Iop *)
@@ -937,24 +937,24 @@ Proof.
   econstructor; eauto.
   (* Icall *)
   assert (wt_fundef fd).
-    destruct ros; simpl in H0.
+    destruct ros; simpl in H1.
     pattern fd. apply Genv.find_funct_prop with unit p (rs#r).
-    exact wt_p. exact H0.
-    caseEq (Genv.find_symbol ge i); intros; rewrite H1 in H0.
+    exact wt_p. exact H1.
+    caseEq (Genv.find_symbol ge i); intros; rewrite H in H1.
     pattern fd. apply Genv.find_funct_ptr_prop with unit p b.
-    exact wt_p. exact H0.
+    exact wt_p. exact H1.
     discriminate.
   econstructor; eauto.
   econstructor; eauto. inv WTI; auto.
   inv WTI. rewrite <- H8. apply wt_regset_list. auto.
   (* Itailcall *)
   assert (wt_fundef fd).
-    destruct ros; simpl in H0.
+    destruct ros; simpl in H1.
     pattern fd. apply Genv.find_funct_prop with unit p (rs#r).
-    exact wt_p. exact H0.
-    caseEq (Genv.find_symbol ge i); intros; rewrite H1 in H0.
+    exact wt_p. exact H1.
+    caseEq (Genv.find_symbol ge i); intros; rewrite H in H1.
     pattern fd. apply Genv.find_funct_ptr_prop with unit p b.
-    exact wt_p. exact H0.
+    exact wt_p. exact H1.
     discriminate.
   econstructor; eauto.
   inv WTI. apply wt_stackframes_change_sig with (fn_sig f); auto.
