cfrontend/Csem.v
@@ -189,6 +189,7 @@ Inductive cast_arguments (m: mem): exprlist -> typelist -> list val -> Prop :=
 Section EXPR.
 
 Variable e: env.
+Variable cp: compartment.
 
 (** The semantics of expressions follows the popular Wright-Felleisen style.
   It is a small-step semantics that reduces one redex at a time.
@@ -298,7 +299,7 @@ Inductive rred: expr -> mem -> trace -> expr -> mem -> Prop :=
         E0 (Eval v ty) m
   | red_builtin: forall ef tyargs el ty m vargs t vres m',
       cast_arguments m el tyargs vargs ->
-      external_call ef ge vargs m t vres m' ->
+      external_call ef ge cp vargs m t vres m' ->
       rred (Ebuiltin ef tyargs el ty) m
          t (Eval vres ty) m'.
 
@@ -631,8 +632,9 @@ Inductive estep: state -> trace -> state -> Prop :=
       estep (ExprState f (C a) k e m)
          E0 (ExprState f (C a') k e m')
 
-  | step_rred: forall C f a k e m t a' m',
-      rred a m t a' m' ->
+  | step_rred: forall cp C f a k e m t a' m',
+      cp = f.(fn_comp) ->
+      rred cp a m t a' m' ->
       context RV RV C ->
       estep (ExprState f (C a) k e m)
           t (ExprState f (C a') k e m')
@@ -644,7 +646,7 @@ Inductive estep: state -> trace -> state -> Prop :=
          E0 (Callstate fd vargs f.(fn_comp) (Kcall f e C ty k) m)
 
   | step_stuck: forall C f a k e m K,
-      context K RV C -> ~(imm_safe e K a m) ->
+      context K RV C -> ~(imm_safe e f.(fn_comp) K a m) ->
       estep (ExprState f (C a) k e m)
          E0 Stuckstate.
 
@@ -792,7 +794,7 @@ Inductive sstep: state -> trace -> state -> Prop :=
          E0 (State f f.(fn_body) k e m2)
 
   | step_external_function: forall ef targs tres cc vargs cp k m vres t m',
-      external_call ef  ge vargs m t vres m' ->
+      external_call ef ge cp vargs m t vres m' ->
       sstep (Callstate (External ef targs tres cc) vargs cp k m)
           t (Returnstate vres k m')
 
@@ -844,7 +846,7 @@ Proof.
   assert (ASSIGN: forall chunk m b ofs t v m', assign_loc ge chunk m b ofs v t m' -> (length t <= 1)%nat).
     intros. inv H0; simpl; try omega. inv H3; simpl; try omega.
   destruct H.
-  inv H; simpl; try omega. inv H0; eauto; simpl; try omega.
+  inv H; simpl; try omega. inv H1; eauto; simpl; try omega.
   eapply external_call_trace_length; eauto.
   inv H; simpl; try omega. eapply external_call_trace_length; eauto.
 Qed.
